newLibrary/finished_examples/readme.md
@@ -23,7 +23,6 @@
 - 5 (windowBloomFilter) will take a while
 - 7 (switchMLFill) will take a while
 
-
 Notes: 
     We could really use external handlers or functions in switchMLSimple or some way to represent multicasting packets (generate_ports).
         - All pretty straightforward to add.
